WIP

cpp/ct2.cpp
@@ -18,59 +18,15 @@
 
 using json = nlohmann::json;
 
+
+std::map<std::string, ctranslate2::Translator> generators;
+std::map<std::string, ctranslate2::Encoder> encoders;
+
 ctranslate2::Translator *p_translator = nullptr;
 ctranslate2::Encoder *p_encoder = nullptr;
 ctranslate2::StorageView *premise_embeddings = nullptr;
 json *premise_dictionary = nullptr;
 
-const std::string EOS_TOKEN = "</s>";
-const std::vector<std::string> byt5_vocab = {
-    "\u0000", "\u0001", "\u0002", "\u0003", "\u0004", "\u0005", "\u0006",
-    "\u0007", "\\b",    "\t",     "\n",     "\u000b", "\\f",    "\r",
-    "\u000e", "\u000f", "\u0010", "\u0011", "\u0012", "\u0013", "\u0014",
-    "\u0015", "\u0016", "\u0017", "\u0018", "\u0019", "\u001a", "\u001b",
-    "\u001c", "\u001d", "\u001e", "\u001f", " ",      "!",      "\"",
-    "#",      "$",      "%",      "&",      "'",      "(",      ")",
-    "*",      "+",      ",",      "-",      ".",      "/",      "0",
-    "1",      "2",      "3",      "4",      "5",      "6",      "7",
-    "8",      "9",      ":",      ";",      "<",      "=",      ">",
-    "?",      "@",      "A",      "B",      "C",      "D",      "E",
-    "F",      "G",      "H",      "I",      "J",      "K",      "L",
-    "M",      "N",      "O",      "P",      "Q",      "R",      "S",
-    "T",      "U",      "V",      "W",      "X",      "Y",      "Z",
-    "[",      "\\",     "]",      "^",      "_",      "`",      "a",
-    "b",      "c",      "d",      "e",      "f",      "g",      "h",
-    "i",      "j",      "k",      "l",      "m",      "n",      "o",
-    "p",      "q",      "r",      "s",      "t",      "u",      "v",
-    "w",      "x",      "y",      "z",      "{",      "|",      "}",
-    "~",      "\u007f", "\u0080", "\u0081", "\u0082", "\u0083", "\u0084",
-    "\u0085", "\u0086", "\u0087", "\u0088", "\u0089", "\u008a", "\u008b",
-    "\u008c", "\u008d", "\u008e", "\u008f", "\u0090", "\u0091", "\u0092",
-    "\u0093", "\u0094", "\u0095", "\u0096", "\u0097", "\u0098", "\u0099",
-    "\u009a", "\u009b", "\u009c", "\u009d", "\u009e", "\u009f", "\u00a0",
-    "\u00a1", "\u00a2", "\u00a3", "\u00a4", "\u00a5", "\u00a6", "\u00a7",
-    "\u00a8", "\u00a9", "\u00aa", "\u00ab", "\u00ac", "\u00ad", "\u00ae",
-    "\u00af", "\u00b0", "\u00b1", "\u00b2", "\u00b3", "\u00b4", "\u00b5",
-    "\u00b6", "\u00b7", "\u00b8", "\u00b9", "\u00ba", "\u00bb", "\u00bc",
-    "\u00bd", "\u00be", "\u00bf", "\u00c0", "\u00c1", "\u00c2", "\u00c3",
-    "\u00c4", "\u00c5", "\u00c6", "\u00c7", "\u00c8", "\u00c9", "\u00ca",
-    "\u00cb", "\u00cc", "\u00cd", "\u00ce", "\u00cf", "\u00d0", "\u00d1",
-    "\u00d2", "\u00d3", "\u00d4", "\u00d5", "\u00d6", "\u00d7", "\u00d8",
-    "\u00d9", "\u00da", "\u00db", "\u00dc", "\u00dd", "\u00de", "\u00df",
-    "\u00e0", "\u00e1", "\u00e2", "\u00e3", "\u00e4", "\u00e5", "\u00e6",
-    "\u00e7", "\u00e8", "\u00e9", "\u00ea", "\u00eb", "\u00ec", "\u00ed",
-    "\u00ee", "\u00ef", "\u00f0", "\u00f1", "\u00f2", "\u00f3", "\u00f4",
-    "\u00f5", "\u00f6", "\u00f7", "\u00f8", "\u00f9", "\u00fa", "\u00fb",
-    "\u00fc", "\u00fd", "\u00fe", "\u00ff"};
-
-std::vector<std::string> byt5_tokenize(const char *input) {
-  std::vector<std::string> tokens;
-  int l = strlen(input);
-  for (int i = 0; i < l; i++) {
-    tokens.push_back(std::string(1, input[i]));
-  }
-  return tokens;
-}
 
 extern "C" uint8_t init_ct2_generator(
     b_lean_obj_arg _model_path,    // String
@@ -119,10 +75,6 @@ std::vector<std::string> convert_tokens(b_lean_obj_arg _tokens) {
 
   for (int i = 0; i < p_arr->m_size; i++) {
     std::string t = lean_string_cstr(p_arr->m_data[i]);
-    if (t != EOS_TOKEN && std::find(byt5_vocab.begin(), byt5_vocab.end(), t) ==
-                              std::end(byt5_vocab)) {
-      throw std::invalid_argument("Invalid token: " + t);
-    }
     tokens.push_back(t);
   }
 
@@ -177,7 +129,6 @@ extern "C" lean_obj_res ct2_generate(
 
   // Get the input tokens ready.
   std::vector<std::string> input_tokens = convert_tokens(_input_tokens);
-  assert(input_tokens.back() == EOS_TOKEN);
   std::vector<std::string> target_prefix_tokens =
       convert_tokens(_target_prefix_tokens);
 
@@ -233,10 +184,6 @@ extern "C" uint8_t is_ct2_encoder_initialized(lean_object *) {
 
 extern "C" lean_obj_res ct2_encode(b_lean_obj_arg _input_tokens) {
   std::vector<std::string> input_tokens = convert_tokens(_input_tokens);
-  // std::vector<std::string> input_tokens = {"n", " ", ":", " ", "\u00e2",
-  // "\u0084", "\u0095", "\n", "\u00e2", "\u008a", "\u00a2", " ", "g", "c", "d",
-  // " ", "n", " ", "n", " ", "=", " ", "n", EOS_TOKEN};
-  assert(input_tokens.back() == EOS_TOKEN);
 
   ctranslate2::EncoderForwardOutput results =
       p_encoder->forward_batch_async({input_tokens}).get();
