LeanCopilot/Models/FFI.lean
@@ -1,4 +1,6 @@
-namespace LeanInfer.FFI
+namespace LeanCopilot
+
+namespace FFI
 
 @[extern "init_ct2_generator"]
 opaque initCt2Generator (modelPath : @& String) (device : @& String) (computeType : @& String) (deviceIndex : @& Array UInt64) (intraThreads : UInt64) : Bool
@@ -35,4 +37,37 @@ opaque isPremiseDictionaryInitialized : Unit → Bool
 @[extern "ct2_retrieve"]
 opaque ct2Retrieve (encodedState : @& Array Float) : Array (String × Float)
 
-end LeanInfer.FFI
+end FFI
+
+
+namespace NativeGenerator
+
+def init (model : NativeGenerator) : Bool :=
+
+
+def generate (model : NativeGenerator) (input : String) : String :=
+
+
+
+  let inputTokens := tokenizeByt5 input true |>.toArray
+  let targetPrefixTokens := tokenizeByt5 targetPrefix false |>.toArray
+  let numReturnSequences := config.decoding.numReturnSequences
+  let beamSize := config.decoding.beamSize
+  let minLength := config.decoding.minLength
+  let maxLength := config.decoding.maxLength
+  let lengthPenalty := config.decoding.lengthPenalty
+  let patience := config.decoding.patience
+  let temperature := config.decoding.temperature
+  let tokensWithScores := FFI.ct2Generate inputTokens targetPrefixTokens numReturnSequences beamSize minLength maxLength lengthPenalty patience temperature
+  tokensWithScores.filterMap fun ((ts, s) : Array String × Float) =>
+    match detokenizeByt5 ts with
+    | "aesop" => none
+    | t => some (t, s)
+
+
+instance : TextToText NativeGenerator where
+  generate := NativeGenerator.generate
+
+end NativeGenerator
+
+end LeanCopilot
