LeanCopilot/LlmAesop.lean
@@ -1,0 +1,17 @@
+import LeanCopilot.Tactics
+import Aesop
+
+open Lean Lean.Elab.Command
+
+namespace LeanCopilot
+
+
+def tacGen : Aesop.TacGen := fun (mvarId : MVarId) => do
+  let state ← ppTacticState [mvarId]
+  generate state ""
+
+
+macro "#init_llm_aesop" : command => `(#eval (initGenerator : IO Bool) @[aesop 100%] def tacGen := LeanCopilot.tacGen #eval getConfig)
+
+
+end LeanCopilot
