LeanCopilot/Models.lean
@@ -1,0 +1,11 @@
+import LeanCopilot.Models.Interface
+import LeanCopilot.Models.Defs
+import LeanCopilot.Models.Registry
+import LeanCopilot.Models.FFI
+
+
+open LeanCopilot
+
+#eval (getModelRegistry : IO _)
+
+#eval generate defaultGenerator "Hi!"
