LeanCopilot/Models/Defs.lean
@@ -1,0 +1,88 @@
+import LeanCopilot.Url
+import LeanCopilot.Models.Interface
+
+set_option autoImplicit false
+
+namespace LeanCopilot
+
+
+inductive Device where
+  | cpu
+  | cuda
+  | auto
+deriving Repr
+
+
+instance : Inhabited Device where
+  default := .auto
+
+
+inductive ComputeType where
+  | default
+  | auto
+  | int8
+  | int8_float32
+  | int8_float16
+  | int8_bfloat16
+  | int16
+  | float16
+  | bfloat16
+  | float32
+deriving Inhabited, Repr
+
+
+instance : Inhabited ComputeType where
+  default := .auto
+
+
+structure Model where
+  isInitialized : Bool := false
+deriving Repr
+
+
+instance : Inhabited Model where
+  default := {}
+
+
+structure NativeModel extends Model where
+  url : HuggingFaceURL
+  device : Device := default
+  deviceIndex : Array UInt64 := #[0]
+  computeType : ComputeType := default
+  hasLocalCopy : Bool := false
+deriving Repr
+
+
+instance : Inhabited NativeModel where
+  default := {url := default}
+
+
+def NativeModel.name (model : NativeModel) : String := model.url.name
+
+
+structure NativeGenerator extends NativeModel
+deriving Repr
+
+
+structure NativeEncoder extends NativeModel
+deriving Repr
+
+
+def NativeEncoder.encode (enc : NativeEncoder) (input : String) : FloatArray :=
+  FloatArray.empty
+
+
+structure ExternalModel extends Model where
+  name : String
+deriving Inhabited, Repr
+
+
+structure ExternalGenerator extends ExternalModel
+deriving Repr
+
+
+structure ExternalEncoder extends ExternalModel
+deriving Repr
+
+
+end LeanCopilot
