LeanCopilot/Models/Interface.lean
@@ -1,0 +1,52 @@
+set_option autoImplicit false
+
+namespace LeanCopilot
+
+
+class TextToText (τ : Type) where
+  generate : τ → String → String
+
+
+class TextToVec (τ : Type) where
+  encode : τ → String → FloatArray
+
+
+def generate {τ : Type} [TextToText τ] (model : τ) (input : String) : String :=
+  TextToText.generate model input
+
+
+def encode {τ : Type} [TextToVec τ] (model : τ) (input : String) : FloatArray :=
+  TextToVec.encode model input
+
+
+structure DummyGenerator where
+  output : String
+
+
+instance : TextToText DummyGenerator where
+  generate model _ := model.output
+
+
+structure DummyEncoder where
+  output : FloatArray
+
+
+instance : TextToVec DummyEncoder where
+  encode model _ := model.output
+
+
+private def gen : DummyGenerator := ⟨"Hello, world!"⟩
+
+
+example : generate gen "Hi!" = "Hello, world!" := by
+  rfl
+
+
+private def enc : DummyEncoder := ⟨FloatArray.mk #[1, 2, 3]⟩
+
+
+example : encode enc "Hi!" = FloatArray.mk #[1, 2, 3] := by
+  rfl
+
+
+end LeanCopilot
