LeanCopilot/Models/Registry.lean
@@ -1,0 +1,61 @@
+import LeanCopilot.Models.Defs
+import Std.Data.HashMap
+
+set_option autoImplicit false
+
+open Std
+
+namespace LeanCopilot
+
+
+def defaultGenerator : NativeGenerator := {
+  url := ⟨"kaiyuy", "ct2-leandojo-lean4-tacgen-byt5-small"⟩
+}
+
+
+def defaultEncoder : NativeEncoder := {
+  url := ⟨"kaiyuy", "ct2-leandojo-lean4-retriever-byt5-small"⟩
+}
+
+
+instance {α β : Type} [BEq α] [Hashable α] [Repr α] [Repr β] : Repr (HashMap α β) where
+  reprPrec hm n := reprPrec hm.toList n
+
+
+structure NativeModelRegistry where
+  generators : HashMap String NativeGenerator :=
+    HashMap.ofList [(defaultGenerator.name, defaultGenerator)]
+  encoders : HashMap String NativeEncoder :=
+    HashMap.ofList [(defaultEncoder.name, defaultEncoder)]
+deriving Repr
+
+
+instance : Inhabited NativeModelRegistry where
+  default := {}
+
+
+structure ExternalModelRegistry where
+  host : String := "localhost"
+  port : UInt16 := 23333
+  generators : HashMap String ExternalGenerator := {}
+  encoders : HashMap String ExternalEncoder := {}
+deriving Repr
+
+
+instance : Inhabited ExternalModelRegistry where
+  default := {}
+
+
+structure ModelRegistry where
+  native : NativeModelRegistry
+  external : ExternalModelRegistry
+deriving Inhabited, Repr
+
+
+initialize modelRegistryRef : IO.Ref ModelRegistry ← IO.mkRef default
+
+
+def getModelRegistry : ST IO.RealWorld ModelRegistry := modelRegistryRef.get
+
+
+end LeanCopilot
