LeanCopilot/Url.lean
@@ -4,22 +4,30 @@ open System (FilePath)
 
 set_option autoImplicit false
 
-namespace LeanInfer
+namespace LeanCopilot
+
 
 def HF_BASE_URL := "https://huggingface.co"
+
 
 structure HuggingFaceURL where
   user : Option String
   modelName : String
 deriving Inhabited
 
+
+def HuggingFaceURL.name : HuggingFaceURL → String
+  | ⟨none, nm⟩ => nm
+  | ⟨some u, nm⟩ => s!"{u}/{nm}"
+
+
 instance : ToString HuggingFaceURL where
-  toString url := match url.user with
-  | none => s!"{HF_BASE_URL}/{url.modelName}"
-  | some user => s!"{HF_BASE_URL}/{user}/{url.modelName}"
+  toString url := s!"{HF_BASE_URL}/{url.name}"
+
 
 instance : Repr HuggingFaceURL where
   reprPrec url x := reprPrec (toString url) x
+
 
 def HuggingFaceURL.isValid (url : HuggingFaceURL) : Bool :=
   let validModelName := ¬ url.modelName.isEmpty ∧ ¬ url.modelName.contains '/'
@@ -28,4 +36,5 @@ def HuggingFaceURL.isValid (url : HuggingFaceURL) : Bool :=
   | some username => ¬ username.isEmpty ∧ ¬ username.contains '/'
   validModelName ∧ validUser
 
-end LeanInfer
+
+end LeanCopilot
