README.md
@@ -1,9 +1,9 @@
-LeanInfer: Native Neural Network Inference in Lean 4
+LeanCopilot: Native Neural Network Inference in Lean 4
 =============================================
 
-<img width="1087" alt="LeanInfer" src="https://github.com/lean-dojo/LeanInfer/assets/5431913/f87ec407-29a5-4468-b2fb-a2f6e9105ae9">
+<img width="1087" alt="LeanCopilot" src="https://github.com/lean-dojo/LeanCopilot/assets/5431913/f87ec407-29a5-4468-b2fb-a2f6e9105ae9">
 
-LeanInfer provides tactic suggestions by running LLMs through Lean's foreign function interface (FFI). It is in an early stage of development. In the long term, we aim to integrate Lean and machine learning by providing a general and efficient way to run the inference of neural networks in Lean. 
+LeanCopilot provides tactic suggestions by running LLMs through Lean's foreign function interface (FFI). It is in an early stage of development. In the long term, we aim to integrate Lean and machine learning by providing a general and efficient way to run the inference of neural networks in Lean. 
 
 
 ## Requirements
@@ -13,32 +13,32 @@ LeanInfer provides tactic suggestions by running LLMs through Lean's foreign fun
 * Optional (recommended if you have a [CUDA-enabled GPU](https://developer.nvidia.com/cuda-gpus)): CUDA and [cuDNN](https://developer.nvidia.com/cudnn)
 
 
-## Adding LeanInfer as a Dependency to Your Project
+## Adding LeanCopilot as a Dependency to Your Project
 
 :warning: Your package must use a Lean version of at least `lean4:v4.3.0-rc2`.
 
-1. Add the package configuration option `moreLinkArgs := #["-L./.lake/packages/LeanInfer/.lake/build/lib", "-lonnxruntime", "-lctranslate2"]` to lakefile.lean. Also add LeanInfer as a dependency:
+1. Add the package configuration option `moreLinkArgs := #["-L./.lake/packages/LeanCopilot/.lake/build/lib", "-lonnxruntime", "-lctranslate2"]` to lakefile.lean. Also add LeanCopilot as a dependency:
 ```lean
-require LeanInfer from git "https://github.com/lean-dojo/LeanInfer.git" @ "v0.0.9"
+require LeanCopilot from git "https://github.com/lean-dojo/LeanCopilot.git" @ "v0.0.9"
 ```
-2. Run `lake update LeanInfer`
-3. Run `lake script run LeanInfer/download` to download the models from Hugging Face to `~/.cache/lean_infer/`
+2. Run `lake update LeanCopilot`
+3. Run `lake script run LeanCopilot/download` to download the models from Hugging Face to `~/.cache/lean_infer/`
 4. Run `lake build`
 
-You may also see the [example here](https://github.com/yangky11/lean4-example/blob/LeanInfer-demo). If you have problems building the project, our [Dockerfile](./Dockerfile), [build.sh](scripts/build.sh) or [build_example.sh](scripts/build_example.sh) may be helpful.
+You may also see the [example here](https://github.com/yangky11/lean4-example/blob/LeanCopilot-demo). If you have problems building the project, our [Dockerfile](./Dockerfile), [build.sh](scripts/build.sh) or [build_example.sh](scripts/build_example.sh) may be helpful.
 
 
-## Using LeanInfer
+## Using LeanCopilot
 
 ### Generating Tactic Suggestions
 
-After `import LeanInfer`, you can use the tactic `suggest_tactics` to generate tactic suggestions (see the image above and [this example](LeanInferTests/Examples.lean)). You can click on any of the suggested tactics to use it in the proof.
+After `import LeanCopilot`, you can use the tactic `suggest_tactics` to generate tactic suggestions (see the image above and [this example](LeanCopilotTests/Examples.lean)). You can click on any of the suggested tactics to use it in the proof.
 
 You may provide a prefix to constrain the generated tactics. For example, `suggest_tactics "rw"` would only generate tactics starting with `rw`.
 
 ### Searching for Proofs
 
-You can combine the LLM-generated tactic suggestions with [aesop](https://github.com/leanprover-community/aesop) to search for complete proofs. To do this, simply add `#init_llm_aesop` before using aesop (see [this example](LeanInferTests/Aesop.lean)). 
+You can combine the LLM-generated tactic suggestions with [aesop](https://github.com/leanprover-community/aesop) to search for complete proofs. To do this, simply add `#init_llm_aesop` before using aesop (see [this example](LeanCopilotTests/Aesop.lean)). 
 
 
 ### Selecting Premises
@@ -46,16 +46,16 @@ You can combine the LLM-generated tactic suggestions with [aesop](https://github
 Coming soon.*
 
 
-## Building LeanInfer
+## Building LeanCopilot
 
-You don't need to build LeanInfer directly if you use it in a downstream package. Nevertheless, if you really need to build LeanInfer, it can be done by `lake build`. However, make sure you have installed these dependencies:
+You don't need to build LeanCopilot directly if you use it in a downstream package. Nevertheless, if you really need to build LeanCopilot, it can be done by `lake build`. However, make sure you have installed these dependencies:
 * CMake >= 3.7
 * A C++17 compatible compiler, e.g., recent versions of GCC or Clang
 
 
 ## Questions and Bugs
 
-* For general questions and discussions, please use [GitHub Discussions](https://github.com/lean-dojo/LeanInfer/discussions).  
+* For general questions and discussions, please use [GitHub Discussions](https://github.com/lean-dojo/LeanCopilot/discussions).  
 * To report a potential bug, please open an issue. In the issue, please include your OS information and the exact steps to reproduce the error. The more details you provide, the better we will be able to help you. 
 
 
@@ -69,7 +69,7 @@ You don't need to build LeanInfer directly if you use it in a downstream package
 ## Acknowledgements
 
 * [llmstep](https://github.com/wellecks/llmstep) is another tool providing tactic suggestions using LLMs. We use their frontend for displaying tactics but a different mechanism for running the model.
-* We thank Scott Morrison for suggestions on simplifying LeanInfer's installation and Mac Malone for helping implement it. Both Scott and Mac work for the [Lean FRO](https://lean-fro.org/).
+* We thank Scott Morrison for suggestions on simplifying LeanCopilot's installation and Mac Malone for helping implement it. Both Scott and Mac work for the [Lean FRO](https://lean-fro.org/).
 * We thank Jannis Limperg for integrating our LLM-generated tactics into aesop (https://github.com/leanprover-community/aesop/pull/70).
 
 
